\section{Question 1}%
\label{sec: Question 1 }
Calculate the iterated integral.
\[
\int_{ 1 }^{ 4 } \int_{ 0 }^{ 2 } \left( 6x^2y-2x \right) dydx
.\] 
Evaluate the inner integral first,
\[
\int_{ 0 }^{ 2 } 6x^2y-2x \, dy = \left[ 3x^2y^2-2xy \right]_{ 0 }^{ 2 } = 12x^2-4x
.\] 
and eval the outer,
\[
\int_{ 1 }^{ 4 } 12x^2-4x \, dx = 4x^3-2x^2 \bigg|_{ 1 }^{ 4 } = 4\left( 64-1 \right) -2\left( 16-1 \right) = 222
.\] 

\section{Question 2}%
\label{sec: Question 2 }
Calculate the double integral.
% horrible way of making the spacing below but like fuck
\[
\int \!\!\!\!\!\int_{ R }^{  } \left( y+xy^{ -2 } \right) dA, R = \left\{ \left( x,y \right) \big|0\le x\le 2, 1 \le y \le 2 \right\} 
.\] 
Based on our region we can write the integral as,
\[
\int_{ 1 }^{ 2 } \int_{ 0 }^{ 2 } \left( y+xy^{ -2 }dx \right) dy \to \int_{ 1 }^{ 2 } \left( yx+\frac{ 1 }{ 2 } x^2y^{ -2 } \bigg|_{ 0 }^{ 2 } \right)dy 
.\] 
\[
=\int_{ 1 }^{ 2 } \left( 2y+2y^{ -2 } \right) dy = y - 2y^{ -1 }\bigg|_{ 1 }^{ 2 }
.\]
\[
= \left( 4-1 \right) - 2\left( \frac{ 1 }{ 2 } -1 \right) =4
.\]
