\section{Question 1}%
\label{sec: Question 1 }
\paragraph{If $ f\left( x,y \right) = \frac{ xy^2 }{ x^2+y^{ 4 } } $ , does $ \lim_{ \left( x,y \right)  \to \left( 0,0 \right) } f\left( x,y \right)  $ exist? \\ \\}
Finding if the limit exists at $ y=x $ ,
\[
\lim_{ \left( x,y \right)  \to \left( 0,0 \right) } \frac{ x^3 }{ x^2\left( 1+x^2 \right)  }= \lim_{ \left( x,y \right)  \to \left( 0,0 \right) } \frac{ x }{ 1+x^2 } =0
.\] 
Now at $ x=y^2 $,
\[
\lim_{ \left( x,y \right)  \to \left( 0,0 \right) } \frac{ y^{ 4 } }{ 2y^{ 4 } } = \frac{ 1 }{ 2 } 
.\] 
\[
\frac{ 1 }{ 2 } \neq 0 \implies \text{ limit does not exist}
.\] 

\section{Question 2}%
\label{sec: Question 2 }
\paragraph{Find the limit, if it exists, or show that the limit does not exist.}
\[
\lim_{ \left( x,y \right)  \to \left( 2,-1 \right) } \frac{ x^2y+xy^2 }{ x^2-y^2 }
.\] 
Applying limits to each term,
\[
\frac{ \left( \displaystyle\lim_{ x \to 2} x^2 \right) + \left( \displaystyle\lim_{ x \to 2} x \cdot \displaystyle\lim_{ y \to -1} y^2 \right)  }{ \displaystyle\lim_{ x \to 2} x^2 - \displaystyle\lim_{ y \to -1} y^2 }= \frac{ \left( 4\cdot \left( -1 \right)  \right) + \left( 2\cdot 1 \right)  }{ 4-1 }= -\frac{ 2 }{ 3 } 
.\] 
Thus our limit exists and is equal to $ -\frac{ 2 }{ 3 } $.

\section{Question 3}%
\label{sec: Question 3 }
\paragraph{Find all the second partial derivatives.}
\[
f\left( x,y \right) = \frac{ y }{ 2x+3y } 
.\] 
Finding the first order partials,
\[
\frac{ \partial f}{\partial x} = \frac{ -2y }{ \left( 2x+3y \right) ^2 }
.\] 
\[
\frac{ \partial f}{\partial y} = \frac{ 2x }{ \left( 2x+3y \right) ^2 }
.\] 

Now onto the second orders, starting with x,
\[
\frac{ \partial^2 f}{\partial x \partial x } = \frac{ \left( 2x+3y \right) ^2\left( 0 \right) - \left( -2y \right) \left( 2\cancel{ \left( 2x+3y \right)  }\left( 2 \right)  \right)  }{ \left( 2x+3y \right) \cancel{ 4 } } = \frac{ 8y }{ \left( 2x+3y \right) ^3 }
.\] 
\[
\frac{ \partial^2 f}{\partial x \partial y} = -\frac{ 2\left( \left( 3y+2x \right) ^2-6y\left( 3y+2x \right)  \right)  }{ \left( 3y+2x \right) ^{ 4 } } = \frac{ 2\left( 3y-2x \right)  }{ \left( 2y+2x \right) ^3 }
.\] 
Second orders with y,
\[
\frac{ \partial^2 f}{\partial y \partial x} = \frac{ \left( 2x+3y \right) ^2 \left( 2 \right) - \left( 2x \right) \left(  \right)  }{ \left( 2x+3y \right) ^{ 4 } } = \frac{ 2\left( 2x+3y \right) ^2  - 8x }{ \left( 2x+3y \right) ^3 }
.\] 
\[
\frac{ \partial^2 f}{\partial y \partial y} = \frac{ \left( 2x+3y \right) ^2\left( 0 \right) - \left( 2x \right) \left( 2\left( 2x+3y \right) \left( 3 \right)  \right)  }{ \left( 3x+3y \right) ^{ 4 } } = \frac{ -12x }{ \left( 2x+3y \right) ^3 }
.\] 

\section{Question 4}%
\label{sec: Question 4 }
\paragraph{Use implicit differentiation to find $ \frac{ \partial z}{\partial x}  $ and $ \frac{ \partial z}{\partial y}  $.}
\[
x^2+2y^2+3z^2=1
.\] 
\[
\frac{ \partial }{\partial x} x^2 + \frac{ \partial }{\partial x} \left( 2y^2 \right) + \frac{ \partial }{\partial x} \left( 3z^2 \right) = \frac{ \partial }{\partial x} 1 \to 2x + 0 + 6z \frac{ \partial z}{\partial x} = 0 \implies \frac{ \partial z}{\partial x} = \frac{ -x }{ 3z }
.\] 
\[
\frac{ \partial }{\partial y} x^2 + \frac{ \partial }{\partial y} \left( 2y^2 \right) + \frac{ \partial }{\partial y} \left( 3z^2 \right) = 0 \to 0 + 4y + 6z \frac{ \partial z}{\partial y} = 0 \implies \frac{ \partial z}{\partial y} = -\frac{ 2y }{ 3z } 
.\] 

