\section{Question 1}%
\label{sec: Question 1 }
\paragraph{Find the domain of the vector function.}
\[
\vec{ r }\left( t \right) = \langle \cos^{  } \left( t \right) , \ln^{  } \left( t \right) , \frac{ 1 }{ t-2 } \rangle
.\] 
$ \ln^{  } \left( t \right)  $ is defined when $ t>0 $ and $ \frac{ 1 }{ t-2 }  $ is defined when $ t \neq 2 $ so our domain is $ \left( 0,2 \right) \cup \left( 2,\infty \right) $
\section{Question 2}%
\label{sec: Question 2 }
\paragraph{Find $ \lim_{ t \to 1} \vec{ r }\left( t \right) =\frac{ t^2-t }{ t-1 }\hat{ i } + \sqrt{ t+8 } \hat{ j } + \frac{ \sin^{  } \left( \pi t \right)  }{ \ln^{  } \left( t \right)  }\hat{ k } $ \\ \\}

Each of these can be evaluated independent of each other so,
\[
\lim_{ t \to 1} \frac{ t^2-t }{ t-1 } \to \lim_{ t \to 1} \frac{ t\cancel{ \left( t-1 \right) }  }{ \cancel{ t-1 } } = t = 1
.\] 
\[
\lim_{ t \to 1} \sqrt{ t+8 } = \sqrt{ 1+8 } = \sqrt{ 9 } = 3
.\] 
\[
\lim_{ t \to 1} \frac{ \sin^{  } \left( \pi t \right)  }{ \ln^{  } \left( t \right)  } = \frac{ 0 }{ 0 } \implies \lim_{ t \to 1} \frac{ \pi \cos^{  } \left( \pi t\right)  }{ \frac{ 1 }{ t }  } = \pi \cos^{  } \left( \pi \right) = -\pi
.\] 
Thus,
\[
\lim_{ t \to 1} \vec{ r }\left( t \right) = \langle 1, 3, -\pi \rangle
.\] 
\section{Question 3}%
\label{sec: Question 3 }
\paragraph{Find the derivative of the vector function.}
\[
\vec{ r }\left( t \right)  = \langle e^{ -t }, t-t^3, \ln^{  } \left( t \right) \rangle
.\] 
Again evaluating each one independent of each other,
\[
\frac{ d }{ dx } e^{ -t } = -e^{ -t }
.\] 
\[
\frac{ d }{ dx } t-t^3 = 1-3t^2
.\] 
\[
\frac{ d }{ dx } \ln^{  } \left( t \right) = \frac{ 1 }{ t } 
.\] 
So,
\[
\frac{ d }{ dx } \vec{ r }\left( t \right) = \langle -e^{ -t }, 1-3t^2, \frac{ 1 }{ t } \rangle
.\] 
\section{Question 4}%
\label{sec: Question 4 }
\paragraph{Find the unit tangent vector $ \vec{ T }\left( t \right)  $ or $ \vec{ r }\left( t \right) = \langle t^2-2t, 1+3t, \frac{ 1 }{ 3 } t^3+\frac{ 1 }{ 2 } t^2 \rangle $ at the point where t = 2 \\ \\}
\[
\vec{ T }\left( t \right) = \frac{ \vec{ r }'\left( t \right)  }{ \left| \vec{ r }
\left( t \right) \right| }
.\] 
\[
r'\left( t \right) = \langle 2t-2, 3, \frac{ 1 }{ 3 } \cdot 3t^2+\frac{ 1 }{ 2 } \cdot 2t \rangle = \langle 2t-2, 3, t^2+t \rangle
.\] 
\[
r'\left( 2 \right) = \langle 2,3,6 \rangle
.\] 
\[
\left| \vec{ r }\left( t \right)  \right| = \sqrt{ 2^2 + 3^2 + 6^2 } = 7 
.\] 
\[
\vec{ T }\left( t \right)  = \frac{ 1 }{ 7 } \langle 2,3,6 \rangle
.\] 
\section{Question 5}%
\label{sec: Question 5 }
\paragraph{Evaluate the integral.}
\[
\int_{ 1 }^{ 4 } \left( 2t^{ \frac{ 3 }{ 2 }  }\hat{ i }+\left( t+1 \right) \sqrt{ t } \hat{ k } \right) dt
.\] 
Simplifying into components,
\[
\int_{ 1 }^{ 4 } 2t^{ \frac{ 3 }{ 2 }  }dt\hat{ i }+\int_{ 1 }^{ 4 } \left( t+1 \right) \sqrt{ t } dt \hat{ k }
.\] 
\[
=\left\langle \frac{ 4 }{ 5 } t^{ \frac{ 5 }{ 2 }  }\bigg|_{ 1 }^{ 4 }, \frac{ 2 }{ 5 } t^{ \frac{ 5 }{ 2 }  }+ \frac{ 2 }{ 3 } t^{ \frac{ 3 }{ 2 }  } \bigg|_{ 1 }^{ 4 } \right\rangle = \left\langle \frac{ 4 }{ 5 } \left( 4^{ \frac{ 5 }{ 2 }  }-1^{ \frac{ 5 }{ 2 }  } \right) , \frac{ 2 }{ 5 } \left( 4^{ \frac{ 5 }{ 2 }  }-1^{ \frac{ 5 }{ 2 }  } \right) + \frac{ 2 }{ 3 }\left( 4^{ \frac{ 3 }{ 2 }  }-1^{ \frac{ 3 }{ 2 }  }\right) \right\rangle = \left\langle \frac{ 124 }{ 5 } , \frac{ 256 }{ 15 } \right\rangle
.\] 
