\section{Question 1}%
\label{sec: Question 1 }
\paragraph{Find the length of the curve}
\[
\vec{ r }\left( t \right) = \langle t, 3\cos^{  } \left( t \right) , 3\sin^{  } \left( t \right) \rangle , -5 \leq t \leq 5
.\] 
\[
L=\int_{ -5 }^{ 5 } \sqrt{ 1^2+9\sin^{ 2 } \left( t \right) +9\cos^{ 2 } \left( t \right)  }  = \int_{ -5 }^{ 5 } \sqrt{ 10 } dt = \sqrt{ 10 } \left( 5- \left( -5 \right)  \right) = 10\sqrt{ 10 }
.\] 

\section{Question 2}%
\label{sec: Question 2}
\paragraph{Find the arc length function for the curve $ \vec{ r }\left( t \right) = \left( 5-t \right) \hat{ i }+\left( 4t-3 \right) \hat{ j } + 3\hat{t}k $ measured from the point $ P\left( 4,1,3 \right)  $ in the direction of increasing t and then reparametrize the curve with respect to arc length starting from P. \\ \\}
\[
5-t = 4 \implies t=1
.\] 
\[
4t-3 = 1 \implies t=1
.\] 
\[
3 =3 \implies t=1 \implies t_0 = 1 \text{ and } t_1 = 4,1,3
.\] 
\[
L=\int_{ 1 }^{ t_1 } \sqrt{ \left( -1 \right) ^2+ \left( 4 \right) ^2+ \left( 3 \right) ^2 } = \int_{ 1 }^{ t_1 } \sqrt{ 26 } du \to L=\sqrt{ 26 } \left( t_1 -1 \right) \implies t = \frac{ L }{ \sqrt{ 26 } } +1
.\] 
\[
r\left( t \right) = r\left( \frac{ L }{ \sqrt{ 26 }  } +1 \right) = \left< 5- \left( \frac{ L }{ \sqrt{ 26 }  } +1 \right), 4\left( \frac{ L }{ \sqrt{ 26 }  } +1 \right) -3, 3\left( \frac{ L }{ \sqrt{ 26 }  } +1 \right)   \right>
.\] 


\section{Question 3}%
\label{sec: Question 3 }
\paragraph{Find the tangent vector.}
\[
\vec{ r }\left( t \right)  = \langle t, 3\cos^{  } \left( t \right) , 3\sin^{  } \left( t \right) \rangle
.\] 
\[
\vec{ r }'\left( t \right) = \langle 1, -3\sin^{  } \left( t \right) , 3\cos^{  } \left( t \right)  \rangle \text{ and } \left| \vec{ r }'\left( t \right)  \right| = \sqrt{ 1^2+9\sin^{ 2 } \left( t \right) + 9\cos^{ 2 } \left( t \right)  }  = \sqrt{ 10 } 
.\] 
\[
\vec{ T }\left( t \right) = \frac{ \vec{ r }'\left( t \right)  }{ \left| \vec{ r }'\left( t \right)  \right| } \implies  \frac{ 1 }{ \sqrt{ 10 } } \langle 1, -3\sin^{  } \left( t \right) , 3\cos^{  } \left( t \right)  \rangle
.\] 

\section{Question 4}%
\label{sec: Question 4 }
\paragraph{Find the curvature}
\[
\vec{ r }\left( t \right) = \left\langle \sqrt{ 2t } , e^{ t }, e^{ -t } \right\rangle
.\] 
\[
\vec{ r }'\left( t \right) = \left< \sqrt{ 2 } , e^{ t }, -e^{ -t } \right> \text{ and } \vec{ r }''\left( t \right) = \left< 0, e^{ t }, e^{ -t } \right>
.\] 
\[
K\left( t \right) = \frac{ \left| \vec{ r }'\left( t \right) \times \vec{ r }''\left( t \right)  \right| }{ \left| \vec{ r }'\left( t \right)  \right|^3 }
.\] 
\[
	\left| \vec{ r }'\left( t \right) \times \vec{ r }''\left( t \right)  \right| = \begin{bmatrix} i & j & k \\ \sqrt{ 2 } & e^{ t } & -e^{ t } \\ 0 & e^{ t } & e^{ -t } \end{bmatrix} = \left< 2,-\sqrt{ 2 } e^{ -t }, \sqrt{ 2 } e^{ t } \right> = \sqrt{ 2^2+\left( \sqrt{ 2 } e^{ -t } \right) ^2 + \left( \sqrt{ 2 } e^{ t } \right) ^2 } = \sqrt{ 4 + 2e^{ -2t }+2e^{ 2t } } 
.\] 
\[
\left| \vec{ r }'\left( t \right)  \right| = \sqrt{ 2+e^{ 2t }+e^{ -2t } } 
.\] 
\[
k\left( t \right) = \frac{ \sqrt{ 4 + 2e^{ -2t }+2e^{ 2t } } }{ \sqrt{ 2+e^{ 2t }+e^{ -2t } } }
.\] 

\section{Question 5}%
\label{sec: Question 5 }
\paragraph{Find the velocity and position vectors of a particle that has the given acceleration and the given initial velocity and position.}
\[
	\mathbf{a}\left( t \right) = 2i + 2t \mathbf{ k } ,  \mathbf{ v } \left( 0 \right) = 3i-j,  \mathbf{ r } \left( 0 \right) = j + k
.\] 
\[
\vec{ v }\left( t \right) = \int_{  }^{  } \vec{ a }\left( t \right)  = \int_{  }^{  } 2\hat{ i }+2\hat{t}k dt =2t \hat{ i } + t^2 \hat{ k } + \vec{ c }
.\] 
Final velocity vector:
\[
	\vec{ c }= 3 \hat{ i } - \hat{ j } \implies \vec{ v }\left( t \right) = \left( 2t+3 \right) \hat{ i } + \left( -1 \right) \hat{ j } + \left( t^2 \right) \hat{ k }
.\] 
Position vector:
\[
\vec{ p }\left( t \right) = \int_{  }^{  } \vec{ v }\left( t \right) dt = \left( t^2 + 3t \right) \hat{ i } + \left( -t \right) \hat{ j } + \left( \frac{ 1 }{ 3 } t^3 \right) \hat{ k } + \vec{ D }	
.\] 
\[
\vec{ p }\left( 0 \right) \vec{ D } = \hat{ j } + \hat{ k }
.\] 
Final pos vector:
\[
\vec{ p }\left( t \right) = \left( t^2 + 3t \right) \hat{ i } + \left( -t + 1  \right) \hat{ j } + \left( \frac{ 1 }{ 3 } t^3 + 1 \right) \hat{ k }
.\] 

