\documentclass[a4paper]{article}

\usepackage[utf8]{inputenc}
\usepackage[T1]{fontenc}
\usepackage{textcomp}
\usepackage[english]{babel}
\usepackage{amsmath, amssymb}
\title{Quiz 4 questions}
\author{yawnbo}
\date{\today}

\maketitle

\pdfsuppresswarningpagegroup=1

\begin{document}
\paragraph{Question 1}
\[
  \tan^{-1}(2x)dx
\]
Start by letting $u=\tan^{-1}(2x)$ and $dv=dx$, so $du=\frac{2}{1+4x^2}$ and $v=x$ \\
We can rewrite the integral as
\[
x\tan^{-1}(2x)-\int_{}^{} \frac{2}{1+4x^2}\cdot xdx
.\]
Where we can now work on the inner integral. Let
\begin{gather*}
  u=1+4x^2 \implies du=8xdx \\
  dx= \frac{1}{8x}du\\
\end{gather*}
The $x$ 's will cancel out and leave us with
\[
-\frac{2}{8}\int_{}^{} \frac{1}{u}du 
.\] 
Which simplifies to
\[
\frac{1}{4}(\ln(1+4x^2))+C
.\] 
At which point we can plug it back into the original expression
\[
x\tan^{-1}(2x)-\frac{1}{4}(\ln(1+4x^2))+C
.\]
\newpage
\paragraph{Question 2}
\[
\int_{0}^{t} e^{8} \sin^{}(t-s)ds
.\]

Begin by simplifying the inside of sin and the exponent of e
\begin{gather*}
  w=t-s \implies dw=-ds \\
  s=t-w \\
  t-0=t \text{ & } t-t=0
\end{gather*}
We need to change the limits and rewrite as
\[
  \int_{t}^{0} e^{t-w}\sin^{}(w)\cdot -dw&= \int_{0}^{t} e^{t-w}\sin^{}(w)dw  \\ 
.\] 
Now we begin to integrate by parts
\begin{gather*}
  u=\sin^{}(w) \implies du=\cos^{}(w)dw \\
  dv=e^{t-w} \implies v=-e^{t-w} 
\end{gather*}
Which gets us to the equation
\[
-\sin^{}(t)-\int_{0}^{t}-e^{t-w}\cos^{}(w)dw
.\]
Doing another IBP will get us to the final step of cyclic equations, so,
\begin{gather*}
  \text{For }\int_{0}^{t} -e^{t-w}\cos^{}(w)dw \\
  u=\cos^{}(w)\implies du=-\sin^{}(w)dw \\
  dv=-e^{t-w}\implies v=e^{t-w} \\
  \cos^{}(t) - e^{t}-\int_{0}^{t} e^{t-w}\cdot -\sin^{}(w)dw =\cos^{}(t)+\int_{0}^{t} e^{t-w}\sin^{}(w)dw \\
\end{gather*}
Which we set equal to the original equation,
\begin{align*}
  \int_{0}^{t} e^{t-w} \sin^{}(w)dw &= -\sin^{}(t)-\cos^{}(t)-e^{t}-\int_{0}^{t} e^{t-w}\sin^{}(w)dw \\
  2\int^{t}_{0}e^{t-w}\sin^{}(w)dw &= -\sin^{}(t)-\cos^{}(t)-e^{t}
\end{align*}
Which finally gets us
\begin{gather*}
  \int_{0}^{t} e^{t-w}\sin^{}(w)dw= \frac{-\sin^{}(t)-\cos^{}(t)-e^{t}}{2} \\
  \text{Or} \\
\int_{0}^{t} e^{t-w}\sin^{}(w)dw= -\frac{\sin^{}(t)+\cos^{}(t)+e^{t}}{2}
\end{gather*}
\newpage
\paragraph{Question 3}

\end{document}
