\documentclass[a4paper]{article}

\usepackage[utf8]{inputenc}
\usepackage[T1]{fontenc}
\usepackage{textcomp}
\usepackage[english]{babel}
\usepackage{amsmath, amssymb}
\title{Quiz 4 questions}
\author{yawnbo}
\date{\today}

\maketitle

\pdfsuppresswarningpagegroup=1

\begin{document}
\paragraph{Question 1}
\[
  \tan^{-1}(2x)dx
\]
Start by letting $u=\tan^{-1}(2x)$ and $dv=dx$, so $du=\frac{2}{1+4x^2}$ and $v=x$ \\
We can rewrite the integral as
\[
x\tan^{-1}(2x)-\int_{}^{} \frac{2}{1+4x^2}\cdot xdx
.\]
Where we can now work on the inner integral. Let
\begin{gather*}
  u=1+4x^2 \implies du=8xdx \\
  dx= \frac{1}{8x}du\\
\end{gather*}
The $x$ 's will cancel out and leave us with
\[
-\frac{2}{8}\int_{}^{} \frac{1}{u}du 
.\] 
Which simplifies to
\[
\frac{1}{4}(\ln(1+4x^2))+C
.\] 
At which point we can plug it back into the original expression
\[
x\tan^{-1}(2x)-\frac{1}{4}(\ln(1+4x^2))+C
.\]
\newpage
\paragraph{Question 2}
\[
\int_{0}^{t} e^{8} \sin^{}(t-s)ds
.\]

Begin by simplifying the inside of sin and the exponent of e
\begin{gather*}
  w=t-s \implies dw=-ds \\
  s=t-w \\
  t-0=t \text{ & } t-t=0
\end{gather*}
We need to change the limits and rewrite as
\[
  \int_{t}^{0} e^{t-w}\sin^{}(w)\cdot -dw&= \int_{0}^{t} e^{t-w}\sin^{}(w)dw  \\ 
.\] 
Now we begin to integrate by parts
\begin{gather*}
  u=\sin^{}(w) \implies du=\cos^{}(w)dw \\
  dv=e^{t-w} \implies v=-e^{t-w} 
\end{gather*}
Which gets us to the equation
\[
-\sin^{}(t)-\int_{0}^{t}-e^{t-w}\cos^{}(w)dw
.\]
Doing another IBP will get us to the final step of cyclic equations, so,
\begin{gather*}
  \text{For }\int_{0}^{t} -e^{t-w}\cos^{}(w)dw \\
  u=\cos^{}(w)\implies du=-\sin^{}(w)dw \\
  dv=-e^{t-w}\implies v=e^{t-w} \\
  \cos^{}(t) - e^{t}-\int_{0}^{t} e^{t-w}\cdot -\sin^{}(w)dw =\cos^{}(t)+\int_{0}^{t} e^{t-w}\sin^{}(w)dw \\
\end{gather*}
Which we set equal to the original equation,
\begin{align*}
  \int_{0}^{t} e^{t-w} \sin^{}(w)dw &= -\sin^{}(t)-\cos^{}(t)-e^{t}-\int_{0}^{t} e^{t-w}\sin^{}(w)dw \\
  2\int^{t}_{0}e^{t-w}\sin^{}(w)dw &= -\sin^{}(t)-\cos^{}(t)-e^{t}
\end{align*}
Which finally gets us
\begin{gather*}
  \int_{0}^{t} e^{s}\sin^{}(t-s)ds= \frac{-\sin^{}(t)-\cos^{}(t)-e^{t}}{2} \\
  \text{Or} \\
\int_{0}^{t} e^{s}\sin^{}(t-s)ds= -\frac{\sin^{}(t)+\cos^{}(t)+e^{t}}{2}
\end{gather*}
\newpage
\paragraph{Question 3}

Find the exact volume obtained by rotating the region bounded by $y=\sin^{2}(x),y=0, \text{ For } x \epsilon[0,\pi^{}]$about the $x-$ axis \\
\\
Start by writing the integral for the area, so,
\[
\pi \int_{0}^{\pi}r^2 \implies \pi \int_{0}^{\pi} \sin^{4}(x)dx 
.\] 
Split the large even power and apply power reduction formulas
\begin{gather*}
\pi^{}\int_{0}^{\pi^{}} \sin^{2}(x)\cdot \sin^{2}(x)dx \\
\pi^{}\int_{0}^{\pi^{}} \frac{1-\cos^{}(2x)}{2}\cdot \frac{1-\cos^{}(2x)}{2}dx
\end{gather*}

Bring constant to the outside and simplify
\[
  \frac{\pi}{4}\int_{0}^{\pi} 1-2\cos^{}(2x)+\cos^{2}(2x)dx
.\] 
Reduce powers again and bring out another $\frac{1}{2}$ 
\[
\frac{\pi}{8}\int_{0}^{\pi } 2-4\cos^{}(2x)+1+\cos^{}(4x)dx
.\]
We can now integrate nicely
\begin{align*}
  &= \frac{\pi}{8}\left( 3x-4\sin^{}(2x)+x+\sin^{}(4x) \right)^{4}_{0} \\
  &= \frac{\pi}{8}[3\pi-0-0] \\
 V &= \frac{3\pi^2}{8} 
.\end{align*}
\newpage
\paragraph{Question 4}

\[
\int_{0}^{2} \sqrt{8-x^2}dx 
.\] 
\end{document}
