\section{Find the Laplace transform for $f\left( x \right) =\cos^{}( ax )$}%
these take WAY too long
\paragraph{Start with our general Laplace transform}
\[
\int_{0}^{\infty} e^{-sx}\cos^{}( ax )dx
.\] 
Do our first IBP by letting
\begin{align*}
  u &= \cos^{}( ax ) \\
  du &= -a\sin^{}( ax ) \\
  v &= -\frac{1}{s}e^{-sx} \\
  dv &= e^{-sx}dx \\
\end{align*}
Rewriting our integral we get
\[
\lim_{T \to \infty} \left(  -\frac{1}{s}e^{-sx}\cos^{}( ax )\big|^{T}_{0}-\int_{0}^{T} -\frac{1}{s}e^{-sx}a\sin^{}( ax )dx\right) 
.\] 
I don't want to clutter this so lets simplify the part before the integral and rewrite the integral by pulling out constants
\begin{align*}
  -\frac{1}{s}e^{-s\left( T \right) }\cos^{}( a\left( T \right) ) &\to \text{ DNE }\\
  -\frac{1}{s}e^{-s\left( 0 \right) }\cos^{}( a\left( 0 \right)  ) &\to \frac{1}{s}
\end{align*}
\[
  \lim_{T \to \infty} \left(  \frac{1}{s}+\int_{0}^{T}\frac{1}{s}e^{-sx}\sin^{}( ax )dx \right) 
.\] 
Again just go back to doing another IBP and rewrite
\begin{align*}
  u &= \sin^{}( ax ) \\
  du &= a\cos^{}( ax ) \\
  v &= -\frac{1}{s}e^{-sx} \\
  dv &= e^{-sx}dx 
\end{align*}
\[
\lim_{T \to \infty} \left( \frac{1}{s}-\frac{a}{s} \left( -\frac{1}{s}e^{-sx}\sin^{}( ax )\big|^{T}_{0}-\int_{0}^{T} -\frac{1}{s}e^{-sx}a\cos^{}( ax )dx \right)  \right) 
.\] 
Again, evaluate inner bounds to find
\[
-\frac{1}{s}e^{-sx}\sin^{}( ax )\big|^{T}_{0} = \text{ DNE }-0
.\] 
Simplify inner integral too and rewrite
\newpage
\[
  \lim_{T \to \infty} \left( \frac{1}{s}-\frac{a}{s}\left( \frac{a}{s}\int_{0}^{T} e^{-sx}\cos^{}( ax )dx \right)  \right) 
.\] 
As a last step simplify the inside and set equal to original expression.
\[
\lim_{T \to \infty}\int_{0}^{T} e^{-sx}\cos^{}( ax )dx=\lim_{T \to \infty} \left( \frac{1}{s}-\frac{a^2}{s^2}\int_{0}^{T} e^{-sx}\cos^{}( ax )dx \right) 
.\] 
Limits cancel and we are left with simple algebra (let $L$ be our integral I'm not writing it 10 times)
\begin{align*}
  &L = \frac{1}{s}-\frac{a^2}{s^2}L \\
  &L\left( 1+\frac{a^2}{s^2} \right) = \frac{1}{s} \\
  &L = \frac{s}{s^2+a^2}.
\end{align*}
