\section*{Tests cont.}%
\label{sec:Tests}
\paragraph{Note that quiz 3 is open by tomorrow and due in a week I assume.}

\paragraph{Ex.}
Apply the ratio test to 
\[
\sum_{ n=0 } ^{ \infty } \left( -1 \right) ^{ n }\frac{ \sqrt{ n} }{ n+1 }
.\] 
Note that our sequence can be called $ a_n $. Now if we sub n for n+1 we can now take the limit,
\[
\lim_{ n \to \infty} \left\| \frac{ a_{ n+1 } }{ a_n } \right\| = \lim_{ n \to \infty} \frac{ \sqrt{ n+1} }{ n+2 }\cdot \frac{ n+1 }{ \sqrt{ n} }= \sqrt{ \frac{ n+1 }{ n }} \cdot \frac{ n+1 }{ n+2 } = 1\cdot 1 = 1
.\] 
Which makes our test inconclusive. This just means that we have to use another test to determine convergence or divergence. \\
Instead looking at our sequence, we can use AST to find that it's monotonically decreasing and that the limit is 0. This means that the series converges by AST. So because $ \frac{ \sqrt{ n} }{ n+1 } $ is monotonically decreasing and $ \lim_{ n \to \infty} \frac{ \sqrt{ n} }{ n+1 } = 0 $, we can say that the series converges by AST.

\paragraph{What if we also wanted to find if the absolute also converges?}
\[
\sum_{ } ^{  } |a_n| = \sum_{  } ^{  } \frac{ \sqrt{ n} }{ n+1 }
.\] 
Comparing to a smaller function $ \sum_{  } ^{  } \frac{ 1 }{ n+1 } $ shows that the series converges by p-test. This means that the series conditionally converges.
\subsection*{11.5.4}%
\label{sub:11.5.4}
\paragraph{The root test }
(i) If $ \lim_{ n \to \infty} \sqrt[ n ]{ \left\| a_n \right\| } <1 $, then $ \sum_{  } ^{  } \left\| a_n \right\| $ converges \\
(ii) If $ \lim_{ n \to \infty} \sqrt[ n ]{ \left\| a_n \right\| } >1 $, then $ \sum_{  } ^{  } a_n $ diverges \\
(iii) If $ \lim_{ n \to \infty} \sqrt[ n ]{ \left\| a_n \right\| } =1 $, then inconclusive. \\ \\ 
\paragraph{Ex.}
\[
\sum_{ n=1 } ^{ \infty } \left( \frac{ n+1 }{ 2n } \right) ^{ n }
.\] 
We commonly use this test when we have something complex to the power of n, so,
\[
\sqrt[ n ]{ \left\| a_n \right\| } =\sqrt[ n ]{ \frac{ n+1 }{ 2n }^{ n } } = \lim_{ n \to \infty} \frac{ n+1 }{ 2n }=\frac{ 1 }{ 2 } < 1
.\] 
Which proves that our sum $ \sum_{  } ^{  } a_n $ converges because its less than 1.

\paragraph{Ex.}
\[
\sum_{ k=1 } ^{ \infty } \left( 1+\frac{ 3 }{ k }  \right) ^{ k^2 }
.\] 
Start by applying the root,
\[
\sqrt[ k ]{ \left\| a_n \right\| } = \sqrt[ k ]{ \left( 1+\frac{ 3 }{ k }  \right) ^{ k^2 } } = \lim_{ n \to \infty}  \left( 1+\frac{ 3 }{ k }  \right) ^{ k }
.\] 
Solving this at the above point makes it indecisive. So we can use the ratio test to find that the series converges. Let our limit equal L, then,
\[
k \ln^{  } \left( 1+\frac{ 3 }{ k }  \right) = \ln^{  } \left( L \right) 
.\] 
Now as $ k \to \infty $ we get an indeterminate form so we can use L'Hopital's rule to get,
\[
k\ln^{  } \left( 1+\frac{ 3 }{ k }  \right) = \frac{ \frac{ 1 }{ 1+\frac{ 3 }{ k }  }\cdot \left( -\frac{ 3 }{ k^2 }  \right)  }{ -\frac{ 1 }{ k^2 }  } = \frac{ 3 }{ 1+\frac{ 3 }{ k }  } \to 3 = \ln^{  } \left( L \right) 
.\] 
So $ L = e^{ 3 } $, which means that the series diverges because $ e^{ 3  }>1 $.
\paragraph{Everything above is done up to section 11.6 and 11.7 is just review on how to actually use these tests}

\paragraph{Example list to do if wanted (compare first to second to prove divergence or convergence)}
\begin{align*}
	1.& \sum_{  } ^{  } \frac{ 1 }{ 5^{ n } } , \sum_{  } ^{  } \frac{ 1 }{ 5^{ n }+n } \\
2.&\sum_{  } ^{  } \frac{ \left( -1 \right) ^{ n } }{ n^{ \frac{ 3 }{ 2 }  } }, \sum_{  } ^{  } \frac{ 1 }{ n^{ \frac{ 3 }{ 2 }  } } \\
3.&\sum_{  } ^{  } \frac{ n }{ r^{ n } } , \sum_{  } ^{  } \frac{ 3^{ n } }{ n } \\
4.&\sum_{  } ^{  } \frac{ n+1 }{ n }, \sum_{  } ^{  } \left( -1 \right) ^{ n } \frac{ n+1 }{ n } \\
5.&\sum_{ n=1 } ^{  } \frac{ n }{ n^2+1 } , \sum_{  } ^{  } \left( \frac{ n }{ n^2+1 }  \right) ^{ n } \\
6.&\sum_{  } ^{  } \frac{ \ln^{  } \left( n \right)  }{ n }, \sum_{ n=10 } ^{  } \frac{ 1 }{ n\ln^{  } \left( n \right)  } \\
7.&\sum_{  } ^{  } \frac{ 1 }{ n+n! } , \sum_{  } ^{  } \left( \frac{ 1 }{ n } +\frac{ 1 }{ n! }  \right) \\
8.&\sum_{  } ^{  } \frac{ 1 }{ \sqrt{ n^2+1} } , \sum_{ } ^{  } \frac{ 1 }{ n\sqrt{ n^2+1} } \\
\end{align*}
